ironfleet/src/IronLockServer/Program.cs
@@ -1,21 +1,103 @@
 ﻿using IronfleetCommon;
+using IronfleetIoFramework;
 using MathNet.Numerics.Distributions;
 using System;
+using System.Collections.Generic;
+using System.IO;
 using System.Linq;
 using System.Numerics;
+using System.Text.Json;
 using System.Threading;
 
 namespace IronLockServer
 {
   class Program
   {
+    static void usage()
+    {
+      Console.Write(@"
+Usage:  dotnet IronLockServer.dll [key=value]...
+
+Allowed keys:
+  service   - file name containing service description
+  private   - file name containing private key
+  verbose   - use verbose output
+");
+    }
+
     static void Main(string[] args)
     {
+      Console.WriteLine("IronLockServer program started");
+
+      Console.WriteLine("Processing command-line arguments");
+
+      Params ps = new Params();
+
+      foreach (var arg in args)
+      {
+        if (!ps.ProcessCommandLineArgument(arg)) {
+          usage();
+          return;
+        }
+      }
+
+      if (!ps.Validate()) {
+        return;
+      }
+
+      string json;
+
+      try {
+        json = File.ReadAllText(ps.ServiceFileName);
+      }
+      catch (Exception e) {
+        Console.WriteLine("ERROR - Could not read contents of service file {0}. Exception:\n{1}", ps.ServiceFileName, e);
+        return;
+      }
+
+      ServiceIdentity serviceIdentity;
+      try {
+        serviceIdentity = JsonSerializer.Deserialize<ServiceIdentity>(json);
+      }
+      catch (Exception e) {
+        Console.WriteLine("ERROR - Could not deserialize contents of service file {0}. Exception:\n{1}",
+                          ps.ServiceFileName, e);
+        return;
+      }
+
+      if (serviceIdentity.ServiceType != "IronLock") {
+        Console.WriteLine("ERROR - Service file {0} contains description of service of type {1}, not IronLock.",
+                          ps.ServiceFileName, serviceIdentity.ServiceType);
+        return;
+      }
+
+      try {
+        json = File.ReadAllText(ps.PrivateKeyFileName);
+      }
+      catch (Exception e) {
+        Console.WriteLine("ERROR - Could not read contents of private key file {0}. Exception:\n{1}", ps.PrivateKeyFileName, e);
+        return;
+      }
+
+      PrivateIdentity privateIdentity;
+      try {
+        privateIdentity = JsonSerializer.Deserialize<PrivateIdentity>(json);
+      }
+      catch (Exception e) {
+        Console.WriteLine("ERROR - Could not deserialize contents of private key file {0}. Exception:\n{1}",
+                          ps.PrivateKeyFileName, e);
+        return;
+      }
+
+      var nc = Native____Io__s_Compile.NetClient.Create(privateIdentity, serviceIdentity.Servers, ps.Verbose);
+      Dafny.ISequence<byte>[] serverPublicKeys =
+        serviceIdentity.Servers.Select(server => Dafny.Sequence<byte>.FromArray(server.PublicKey)).ToArray();
+      var ironArgs = Dafny.Sequence<Dafny.ISequence<byte>>.FromArray(serverPublicKeys);
+
       Profiler.Initialize();
       Native____Io__s_Compile.Time.Initialize();
-      Console.WriteLine("IronFleet program started.");
       Console.WriteLine("[[READY]]");
-      Main__i_Compile.__default._Main();
+      Main__i_Compile.__default.IronfleetMain(nc, ironArgs);
       Console.WriteLine("[[EXIT]]");
     }
   }
