ironfleet/src/Dafny/Distributed/Impl/Lock/CmdLineParser.i.dfy
@@ -18,110 +18,40 @@ function lock_config_parsing(args:seq<seq<byte>>) : seq<EndPoint>
     []
 }
 
-function lock_cmd_line_parsing(env:HostEnvironment) : (seq<EndPoint>, EndPoint)
-  reads env
-  reads env.constants
-{
-  var args := env.constants.CommandLineArgs();
-  if |args| < 1 then
-    ([], EndPoint([])) 
-  else
-    var final_arg := args[|args|-1];
-    var config := lock_config_parsing(args[..|args|-1]);
-    var (_, me) := parse_end_point(final_arg);
-    (config, me)
-}
-
-method GetHostIndex(host:EndPoint, hosts:seq<EndPoint>) returns (found:bool, index:uint64)
-  requires EndPointIsValidPublicKey(host)
-  requires SeqIsUnique(hosts)
-  requires |hosts| < 0x1_0000_0000_0000_0000
-  requires forall h :: h in hosts ==> EndPointIsValidPublicKey(h)
-  ensures  found ==> 0 <= index as int < |hosts| && hosts[index] == host
-  ensures !found ==> !(host in hosts)
-{
-  var i:uint64 := 0;
-
-  while i < (|hosts| as uint64)
-    invariant i as int <= |hosts|;
-    invariant forall j :: 0 <= j < i ==> hosts[j] != host;
-  {
-    if host == hosts[i] {
-      found := true;
-      index := i;
-    
-      calc ==> {
-        true;
-          { reveal_SeqIsUnique(); }
-        forall j :: 0 <= j < |hosts| && j != i as int ==> hosts[j] != host;
-      }
-
-      return;
-    }
-
-    if i == (|hosts| as uint64) - 1 {
-      found := false;
-      return;
-    }
-
-    i := i + 1;
-  }
-  found := false;
-}
-
-method ParseCmdLine(ghost env:HostEnvironment) returns (ok:bool, host_ids:seq<EndPoint>, my_index:uint64)
-  requires HostEnvironmentIsValid(env)
-  ensures ok ==> |host_ids| > 0
-  ensures ok ==> 0 <= my_index as int < |host_ids|
-  ensures var (host_ids', my_ep') := lock_cmd_line_parsing(env);
-          ok ==> host_ids == host_ids' && host_ids[my_index] == my_ep'
-  ensures var args := env.constants.CommandLineArgs();
-          ok ==> |args| > 0 && host_ids[my_index] == EndPoint(args[|args|-1])
-  ensures ok ==> SeqIsUnique(host_ids)
+method ParseCmdLine(id:EndPoint, args:seq<seq<byte>>)
+  returns (ok:bool, host_ids:seq<EndPoint>, my_index:uint64)
+  requires EndPointIsValidPublicKey(id)
+  ensures ok ==> && 0 <= my_index as int < |host_ids|
+                && host_ids == lock_config_parsing(args)
+                && host_ids[my_index] == id
+                && SeqIsUnique(host_ids)
 {
   ok := false;
-  var num_args := HostConstants.NumCommandLineArgs(env);
-  var args := collect_cmd_line_args(env);
-  assert args == env.constants.CommandLineArgs();
 
-  if |args| < 1 {
-    print "Incorrect number of command line arguments.\n";
-    print "Expected: ./Main.exe [public_key]+ [public_key]\n";
-    print "  where the final argument is one of the public keys provided earlier \n";
+  var tuple1 := parse_end_points(args);
+  ok := tuple1.0;
+  if !ok {
     return;
   }
-
-  var tuple1 := parse_end_points(args[..|args|-1]);
-  ok := tuple1.0;
-  var endpoints := tuple1.1;
-  if !ok || |endpoints| == 0 || |endpoints| >= 0x1_0000_0000_0000_0000 {
+  host_ids := tuple1.1;
+  if |host_ids| == 0 || |host_ids| >= 0x1_0000_0000_0000_0000 {
     ok := false;
     return;
   }
 
-  var tuple2 := parse_end_point(args[|args|-1]);
-  ok := tuple2.0;
-  if !ok {
-    return;
-  }
-
-  var unique := test_unique(endpoints);
+  var unique := test_unique(host_ids);
   if !unique {
     ok := false;
     return;
   }
 
-  ok, my_index := GetHostIndex(tuple2.1, endpoints);
+  ok, my_index := GetHostIndex(id, host_ids);
   if !ok {
     return;
   }
-  host_ids := endpoints;
-  var me := endpoints[my_index];
 
-  ghost var ghost_tuple := lock_cmd_line_parsing(env);
-  ghost var config', my_ep' := ghost_tuple.0, ghost_tuple.1;
-  assert endpoints == config';
-  assert me == my_ep';
+  ghost var ghost_host_ids := lock_config_parsing(args);
+  assert host_ids == ghost_host_ids;
 }
 
 }
